Adapt proof of NSL.

nsl.v
@@ -12,6 +12,7 @@ Unset Printing Implicit Defensive.
 Section NSL.
 
 Context `{!cryptoG Σ, !heapG Σ}.
+Notation iProp := (iProp Σ).
 
 Implicit Types t : term.
 Implicit Types SM : gmap term session_data.
@@ -19,8 +20,8 @@ Implicit Types s : session_data.
 Implicit Types lvl : level.
 
 Class nslG := {
-  in_nsl_sessG :> inG Σ (authR session_mapUR);
-  nsl_sess_name : gname;
+  in_nsl_sessG :> sessionG Σ;
+  nsl_name : gname;
 }.
 
 Context `{!tagG Σ, !nslG}.
@@ -28,9 +29,9 @@ Context `{!tagG Σ, !nslG}.
 Definition msg1_spec nA pkA :=
   TPair (TInt 1) (TPair nA (TPair pkA (TInt 0))).
 
-Definition msg1_pred p : iProp Σ :=
+Definition msg1_pred p : iProp :=
   ∃ nA kA, ⌜p.2 = Spec.of_list [nA; TKey Enc kA]⌝ ∗
-           session_frag nA (SessionData Init kA p.1 None).
+           session_frag nsl_name nA (SessionData Init kA p.1 None).
 
 Global Instance msg1_pred_proper : NonExpansive msg1_pred.
 Proof.
@@ -40,10 +41,10 @@ Qed.
 Global Instance msg1_pred_persistent p : Persistent (msg1_pred p).
 Proof. apply _. Qed.
 
-Definition msg2_pred p : iProp Σ :=
+Definition msg2_pred p : iProp :=
   ∃ nA nB kB,
     ⌜p.2 = Spec.of_list [nA; nB; TKey Enc kB]⌝ ∗
-    term_session_frag nB (Session Resp p.1 kB (Some nA)).
+    session_frag nsl_name nB (SessionData Resp p.1 kB (Some nA)).
 
 Global Instance msg2_pred_proper : NonExpansive msg2_pred.
 Proof.
@@ -58,10 +59,10 @@ case: p=> kA t.
 case: t; try by move=> *; apply _.
 Qed.
 
-Definition msg3_pred p : iProp Σ :=
+Definition msg3_pred p : iProp :=
   ∃ nA kA,
-    term_session_frag nA (Session Init kA p.1 (Some p.2)) ∗
-    term_session_frag p.2 (Session Resp kA p.1 (Some nA)).
+    session_frag nsl_name nA (SessionData Init kA p.1 (Some p.2)) ∗
+    session_frag nsl_name p.2 (SessionData Resp kA p.1 (Some nA)).
 
 Global Instance msg3_pred_proper : NonExpansive msg3_pred.
 Proof.
@@ -72,10 +73,7 @@ Qed.
 Global Instance msg3_pred_persistent p : Persistent (msg3_pred p).
 Proof. apply _. Qed.
 
-Definition role_name rl : gname :=
-  if rl is Init then nsl_init_name else nsl_resp_name.
-
-Definition nsl_key rl k : iProp Σ :=
+Definition nsl_key_inv rl k : iProp :=
   termT Pub (TKey Enc k) ∗
   stermT Sec (TKey Dec k) ∗
   match rl with
@@ -83,240 +81,22 @@ Definition nsl_key rl k : iProp Σ :=
   | Resp => tkey_predT "m1" (OfeMor msg1_pred) k ∗
             tkey_predT "m3" (OfeMor msg3_pred) k
   end.
-Arguments nsl_key : simpl never.
+Arguments nsl_key_inv : simpl never.
 
-Global Instance nsl_key_persistent rl k :
-  Persistent (nsl_key rl k).
-Proof. rewrite /nsl_key; case: rl; apply _. Qed.
+Global Instance nsl_key_inv_persistent rl k :
+  Persistent (nsl_key_inv rl k).
+Proof. rewrite /nsl_key_inv; case: rl; apply _. Qed.
 
-Lemma nsl_key_pub rl k : nsl_key rl k -∗ termT Pub (TKey Enc k).
+Lemma nsl_key_inv_pub rl k : nsl_key_inv rl k -∗ termT Pub (TKey Enc k).
 Proof. by iDestruct 1 as "[??]". Qed.
 
-Definition coherent_views SM t1 s1 : Prop :=
-  match s1.(srole), s1.(sdata) with
-  | Init, None => True
-  | Init, Some t2 =>
-    SM !! t2 = Some (Session Resp s1.(sinit) s1.(sresp) (Some t1))
-  | Resp, None => False
-  | Resp, Some _ => True
-  end.
+Definition nsl_inv : iProp :=
+  session_inv nsl_name (cryptoN.@"nsl") nsl_key_inv.
 
-Definition session_inv SM : iProp Σ :=
-  ∀ t1 s1, ⌜SM !! t1 = Some s1⌝ -∗
-    nsl_key s1.(srole) (sowner s1)
-    ∗ nsl_key (sroleo s1) (sother s1)
-    ∗ crypto_meta t1 (cryptoN.@"nsl") ()
-    ∗ stermT Sec t1
-    ∗ (if sdata s1 is Some t2 then stermT Sec t2 else True)
-    ∗ ⌜coherent_views SM t1 s1⌝.
+Definition nsl_ctx : iProp :=
+  session_ctx nsl_name (cryptoN.@"nsl") nsl_key_inv.
 
-Global Instance session_inv_persistent SM : Persistent (session_inv SM).
-Proof. apply _. Qed.
-
-Lemma session_inv_unregistered SM t :
-  crypto_meta_token t (↑cryptoN.@"nsl") -∗
-  session_inv SM -∗
-  ⌜SM !! t = None⌝.
-Proof.
-iIntros "Hunreg Hinv".
-destruct (SM !! t) as [s_t|] eqn:SM_t=> //.
-iDestruct ("Hinv" $! _ _ SM_t) as "(?&?&Hreg&?)".
-by iDestruct (crypto_meta_meta_token with "Hunreg Hreg") as "[]".
-Qed.
-
-Definition nsl_inv : iProp Σ :=
-  auth_inv nsl_sess_name to_session_map session_inv.
-
-Definition nsl_ctx : iProp Σ :=
-  auth_ctx nsl_sess_name (cryptoN.@"nsl") to_session_map session_inv.
-
-Lemma nsl_sess_alloc lvl kI kR t rl E ot :
-  let kA := if rl is Init then kI else kR in
-  let kB := if rl is Init then kR else kI in
-  let s  := Session rl kI kR ot           in
-  ↑cryptoN.@"nsl" ⊆ E →
-  (if rl is Init then ot = None else is_Some ot) →
-  nsl_ctx -∗
-  nsl_key rl kA -∗
-  crypto_meta_token t (↑cryptoN.@"nsl") -∗
-  termT Pub (TKey Enc kB) -∗
-  guarded lvl (nsl_key (swap_role rl) kB) -∗
-  stermT lvl t -∗
-  (if ot is Some t' then stermT lvl t' else True) ={E}=∗
-  guarded lvl (term_session_auth t s ∗ term_session_frag t s).
-Proof.
-move=> kA kB s sub rl_ot; iIntros "#Hctx #Howner Hunreg #HkB #HkB' #Ht #Ht'".
-case: lvl => //=.
-iMod (auth_empty nsl_sess_name) as "#Hinit".
-iMod (auth_acc to_session_map session_inv
-         with "[Hctx Hinit]") as "Hinv"; try by eauto.
-iDestruct "Hinv" as (SM) "(_ & Hinv & Hclose)".
-iAssert (▷ ⌜SM !! t = None⌝)%I as "# > %Hfresh".
-  iModIntro.
-  by iApply (session_inv_unregistered with "[Hunreg] [Hinv]").
-iMod (crypto_meta_set _ () with "Hunreg") as "#Hreg"; eauto.
-rewrite -auth_own_op singleton_op.
-iApply ("Hclose" $! (<[t:=s]>SM)); iSplit.
-  iPureIntro. rewrite /to_session_map fmap_insert.
-  apply alloc_singleton_local_update.
-    by rewrite lookup_fmap Hfresh.
-  by apply session_valid.
-iIntros "!>" (t1' s1').
-case: (decide (t = t1')) => [<-|ne].
-  rewrite lookup_insert.
-  iIntros (Hs); case: Hs=> {s1'}<-.
-  do 5![iSplit=> //].
-  rewrite /s; case: (rl) rl_ot=> // rl_ot.
-    by rewrite rl_ot.
-  by case: rl_ot=> t' -> /=.
-rewrite lookup_insert_ne //; iIntros (SM_t1').
-iDestruct ("Hinv" $! _ _ SM_t1') as "(? & ? & ? & ? & ? & %Hcoh)".
-iFrame; iPureIntro.
-move: Hcoh; rewrite /coherent_views.
-case: (srole s1') (sdata s1')=> [|] [t2'|] //.
-case: (decide (t = t2'))=> [<-|?]; first by rewrite Hfresh.
-by rewrite lookup_insert_ne.
-Qed.
-
-Lemma nsl_sess_alloc_init lvl kA kB tA E :
-  ↑cryptoN.@"nsl" ⊆ E →
-  nsl_ctx -∗
-  nsl_key Init kA -∗
-  crypto_meta_token tA (↑cryptoN.@"nsl") -∗
-  termT Pub (TKey Enc kB) -∗
-  guarded lvl (nsl_key Resp kB) -∗
-  stermT lvl tA ={E}=∗
-  guarded lvl (term_session_auth tA (Session Init kA kB None) ∗
-               term_session_frag tA (Session Init kA kB None)).
-Proof.
-iIntros (HE) "#Hctx #HkA Hunreg #HkB #HkB' #HtA".
-by iApply (nsl_sess_alloc with "Hctx HkA Hunreg HkB HkB' HtA").
-Qed.
-
-Lemma nsl_sess_alloc_resp lvl kA kB tA tB E :
-  ↑cryptoN.@"nsl" ⊆ E →
-  nsl_ctx -∗
-  nsl_key Resp kB -∗
-  crypto_meta_token tB (↑cryptoN.@"nsl") -∗
-  termT Pub (TKey Enc kA) -∗
-  guarded lvl (nsl_key Init kA) -∗
-  stermT lvl tB -∗
-  stermT lvl tA ={E}=∗
-  guarded lvl (term_session_auth tB (Session Resp kA kB (Some tA)) ∗
-               term_session_frag tB (Session Resp kA kB (Some tA))).
-Proof.
-iIntros (?) "#Hctx #HkB Hunreg #HkA #HkA' #HtB #HtA".
-by iApply (nsl_sess_alloc with "Hctx HkB Hunreg HkA HkA' HtB")=> /=; eauto.
-Qed.
-
-Lemma session_map_auth_included t s SM :
-  {[t := session_auth s]} ≼ to_session_map SM ↔
-  SM !! t = Some s.
-Proof.
-split.
-- move=> e; apply/leibniz_equiv.
-  case/singleton_included_l: e=> x [].
-  rewrite lookup_fmap option_equivE.
-  case: (SM !! t)=> [s'|] //= <-.
-  rewrite Some_included; case.
-  + by case=> /= _; rewrite option_equivE.
-  + by rewrite session_auth_included=> <-.
-- move=> e; apply/singleton_included_l.
-  exists (session_auth_frag s).
-  by rewrite lookup_fmap e /= Some_included session_auth_included; eauto.
-Qed.
-
-Lemma session_map_frag_included t s SM :
-  {[t := session_frag s]} ≼ to_session_map SM ↔
-  ∃ s', SM !! t = Some s' ∧ to_session s ≼ to_session s'.
-Proof.
-split.
-- case/singleton_included_l=> x [].
-  rewrite lookup_fmap option_equivE.
-  case: (SM !! t)=> [s'|] //= <-.
-  rewrite Some_included; case.
-  + by case=> /=; rewrite option_equivE.
-  + rewrite session_frag_included; eauto.
-- case=> s' [H1 H2].
-  apply/singleton_included_l.
-  rewrite lookup_fmap H1 /=.
-  exists (session_auth_frag s'); split=> //.
-  by rewrite Some_included session_frag_included; right.
-Qed.
-
-Lemma term_session_nsl_key E lvl t s :
-  ↑cryptoN.@"nsl" ⊆ E →
-  nsl_ctx -∗
-  guarded lvl (term_session_frag t s) ={E}=∗
-  ▷ guarded lvl (nsl_key s.(srole) (sowner s)).
-Proof.
-move=> sub; iIntros "#Hctx Hterm"; case: lvl => //=.
-iMod (auth_acc to_session_map _ _ _ _ {[t := session_frag s]}
-         with "[Hctx Hterm]") as "Hinv"; try by eauto.
-iDestruct "Hinv" as (SM) "(%Hincl & Hinv & Hclose)".
-iAssert (▷ nsl_key s.(srole) (sowner s))%I with "[Hinv]" as "#Hs".
-  case/session_map_frag_included: Hincl=> s' [SM_t ss'].
-  iModIntro.
-  rewrite /sowner; case/to_session_included: ss'=> -> [-> [-> _]].
-  by iDestruct ("Hinv" $! _ _ SM_t) as "(?&?&?&?&?&?)".
-by iMod ("Hclose" $! SM {[t := session_frag s]} with "[Hinv]"); eauto.
-Qed.
-
-Definition session_inv' t1 s1 : iProp Σ :=
-  nsl_key s1.(srole) (sowner s1)
-  ∗ nsl_key (sroleo s1) (sother s1)
-  ∗ crypto_meta t1 (cryptoN.@"nsl") ()
-  ∗ stermT Sec t1
-  ∗ (if sdata s1 is Some t2 then stermT Sec t2 else True).
-
-Lemma term_session_session_inv0 E lvl t s :
-  ↑cryptoN.@"nsl" ⊆ E →
-  nsl_ctx -∗
-  guarded lvl (term_session_frag t s) ={E}=∗
-  ∃ s', ⌜to_session s ≼ to_session s'⌝ ∗ ▷ guarded lvl (session_inv' t s').
-Proof.
-move=> sub; iIntros "#Hctx Hterm"; case: lvl => //=.
-  by iExists s.
-iMod (auth_acc to_session_map session_inv
-         with "[Hctx Hterm]") as "Hinv"; try by eauto.
-iDestruct "Hinv" as (SM) "(%Hincl & #Hinv & Hclose)".
-case/session_map_frag_included: Hincl=> s' [SM_t ss'].
-iExists s'.
-iAssert (▷ session_inv' t s')%I with "[Hinv]" as "#Hs".
-  iModIntro.
-  iDestruct ("Hinv" $! _ _ SM_t) as "(?&?&?&?&?&?)".
-  by iSplit => //; eauto.
-by iMod ("Hclose" $! SM {[t := session_frag s]} with "[Hinv]"); eauto.
-Qed.
-
-Lemma term_session_session_inv1 E lvl rl kA kB t t' :
-  ↑cryptoN.@"nsl" ⊆ E →
-  let s := Session rl kA kB (Some t') in
-  nsl_ctx -∗
-  guarded lvl (term_session_frag t s) ={E}=∗
-  ▷ guarded lvl (session_inv' t s).
-Proof.
-move=> sub s; iIntros "#Hctx #Hterm".
-iMod (term_session_session_inv0 with "Hctx Hterm") as (s') "[%s_s' Hs']" => //.
-do 2!iModIntro.
-rewrite /session_inv' /sowner /sother /sroleo /=.
-by case/to_session_included: s_s' => <- [] <- [] <- <- /=.
-Qed.
-
-Lemma term_session_session_inv2 E lvl t s :
-  ↑cryptoN.@"nsl" ⊆ E →
-  nsl_ctx -∗
-  termT lvl t -∗
-  guarded lvl (term_session_frag t s) ={E}=∗
-  ▷ stermT lvl t.
-Proof.
-iIntros (sub) "#Hctx #Ht #Hsess".
-iMod (term_session_session_inv0 with "Hctx Hsess") as (s') "[%s_s' Hs']" => //.
-iDestruct "Hs'" as "(_&_&_&#Ht'&_)".
-by case: lvl=> //=; do 2!iModIntro; iSplit; eauto.
-Qed.
-
-Lemma term_session_session_inv3 E lvl t s :
+(*Lemma term_session_session_inv3 E lvl t s :
   ↑cryptoN.@"nsl" ⊆ E →
   nsl_ctx -∗
   termT lvl (TKey Enc (sowner s)) -∗
@@ -330,88 +110,7 @@ case: lvl=> //=; do 2!iModIntro.
 rewrite /sowner.
 case/to_session_included: s_s' => [] <- [] <- [] <- _.
 by iApply nsl_key_pub.
-Qed.
-
-Lemma term_session_session_inv4 E lvl t s :
-  ↑cryptoN.@"nsl" ⊆ E →
-  nsl_ctx -∗
-  guarded lvl (term_session_frag t s) ={E}=∗
-  ▷ guarded lvl (nsl_key (srole s) (sowner s)).
-Proof.
-iIntros (sub) "#Hctx #Hsess".
-iMod (term_session_session_inv0 with "Hctx Hsess") as (s') "[%s_s' Hs']" => //.
-iDestruct "Hs'" as "(#Hk&_)".
-case: lvl=> //=; do 2!iModIntro.
-rewrite /sowner.
-by case/to_session_included: s_s' => [] <- [] <- [] <- _.
-Qed.
-
-Arguments sroleo !_ /.
-Arguments sother !_ /.
-Arguments sowner !_ /.
-
-Lemma nsl_sess_update lvl kA kB tA tB E :
-  ↑cryptoN.@"nsl" ⊆ E →
-  nsl_ctx -∗
-  guarded lvl (term_session_auth tA (Session Init kA kB None)) -∗
-  guarded lvl (term_session_frag tB (Session Resp kA kB (Some tA))) ={E}=∗
-  guarded lvl (term_session_auth tA (Session Init kA kB (Some tB)) ∗
-               term_session_frag tA (Session Init kA kB (Some tB))).
-Proof.
-iIntros (sub) "Hctx HA HB"; case: lvl => //=.
-case: (decide (tA = tB))=> [<-|tAB].
-  iPoseProof (term_session_agree with "HA HB") as "%agree".
-  by rewrite to_session_included /= in agree *; intuition.
-set s1 := Session Init _ _ _; set s2 := Session Resp _ _ _.
-pose (f1 := {[tA := session_auth s1]} : gmap _ _).
-pose (f2 := {[tB := session_frag s2]} : gmap _ _).
-iMod (auth_acc to_session_map _ _ _ _
-         (f1 ⋅ f2) with "[Hctx HA HB]") as "Hinv"; try by eauto.
-  by rewrite auth_own_op; iFrame.
-iDestruct "Hinv" as (SM) "(%Hincl & #Hinv & Hclose)".
-have /session_map_auth_included SM_tA : f1 ≼ to_session_map SM.
-  apply: cmra_included_trans Hincl; exact: cmra_included_l.
-have /session_map_frag_included SM_tB: f2 ≼ to_session_map SM.
-  apply: cmra_included_trans Hincl; exact: cmra_included_r.
-case: SM_tB=> s2' [SM_tB s2_incl].
-move: SM_tB; rewrite -(to_session_included_eq s2_incl) /=; last by eauto.
-move=> SM_tB {s2' s2_incl}.
-set s1' := Session Init kA kB (Some tB).
-pose (f1' := {[tA := session_auth_frag s1']} : gmap _ _).
-pose (SM' := <[tA := s1']> SM).
-iMod ("Hclose" $! (<[tA := s1']>SM) (f1' ⋅ f2) with "[]") as "Hown"; last first.
-  rewrite /f1' -singleton_op !auth_own_op; iModIntro.
-  by iDestruct "Hown" as "[[??]?]"; iFrame.
-have f2_tA : f2 !! tA = None by rewrite lookup_singleton_ne.
-iSplit.
-  iPureIntro.
-  rewrite /to_session_map fmap_insert -![_ ⋅ f2]insert_singleton_op //.
-  rewrite -(insert_insert f2 tA (session_auth_frag s1') (session_auth s1)).
-  eapply insert_local_update.
-  - by rewrite lookup_fmap SM_tA.
-  - by rewrite lookup_insert.
-  apply local_update_unital_discrete.
-  intros a _ <-%cancelable=> //; last by apply _.
-  split=> //; first exact: session_auth_frag_valid.
-  rewrite {2}/session_auth_frag -cmra_assoc -auth_frag_op -Some_op.
-  by rewrite /to_session /= -!pair_op !agree_idemp.
-iIntros "!>" (t s).
-case: (decide (tA = t))=> [<-|ne].
-  rewrite lookup_insert; iIntros (e); case: e=> ?; subst s.
-  iDestruct ("Hinv" $! _ _ SM_tA) as "(?&?&?&?&?&?)".
-  iDestruct ("Hinv" $! _ _ SM_tB) as "(?&?&?&?&?&?)".
-  do 5![iSplit=> //]; iPureIntro.
-  rewrite /s1' /=.
-  by rewrite /coherent_views /= lookup_insert_ne // SM_tB.
-rewrite lookup_insert_ne //.
-iIntros "%SM_t"; iDestruct ("Hinv" $! _ _ SM_t) as "(?&?&?&?&?&%Hcoh)".
-do 5![iSplit=> //]; iPureIntro.
-move: Hcoh; rewrite /coherent_views.
-case erole: (srole s)=> //.
-case edata: (sdata s)=> [t'|] //.
-case: (decide (tA = t'))=> [<-|?]; first by rewrite SM_tA.
-by rewrite lookup_insert_ne.
-Qed.
+Qed.*)
 
 Variable send recv gen : val.
 
@@ -446,7 +145,7 @@ Definition responder (skB pkB : val) : val := λ: <>,
     if: eq_term "m3" "nB" then SOME ("pkA", "nA", "nB") else NONE
   else NONE.
 
-Implicit Types Ψ : val → iProp Σ.
+Implicit Types Ψ : val → iProp.
 
 Hypothesis wp_send : forall E t Ψ,
   ▷ termT Pub t -∗
@@ -464,11 +163,11 @@ Hypothesis wp_gen : forall E lvl Ψ,
   WP gen #() @ E {{ Ψ }}.
 
 Lemma termT_msg1 lvl kA kB (tA : term) :
-  nsl_key Init kA -∗
+  nsl_key_inv Init kA -∗
   stermT lvl tA -∗
   termT Pub (TKey Enc kB) -∗
-  guarded lvl (nsl_key Resp kB) -∗
-  guarded lvl (term_session_frag tA (Session Init kA kB None)) -∗
+  guarded lvl (nsl_key_inv Resp kB) -∗
+  guarded lvl (session_frag nsl_name tA (SessionData Init kA kB None)) -∗
   termT Pub (TEnc kB (Spec.tag "m1" (Spec.of_list [tA; TKey Enc kA]))).
 Proof.
 iIntros "#HkA #HtA #HkB_lo (#HkB_hi & #HkB_hi' & #? & _) #frag".
@@ -486,15 +185,15 @@ Lemma wp_initiator kA kB (tA : term) lvl E Ψ :
   nsl_ctx -∗
   stermT lvl tA -∗
   crypto_meta_token tA (↑cryptoN.@"nsl") -∗
-  nsl_key Init kA -∗
+  nsl_key_inv Init kA -∗
   termT Pub (TKey Enc kB) -∗
-  guarded lvl (nsl_key Resp kB) -∗
+  guarded lvl (nsl_key_inv Resp kB) -∗
   (∀ onB : option term,
       (if onB is Some tB then
          stermT lvl tB ∗
          guarded lvl (
-           term_session_auth tA (Session Init kA kB (Some tB)) ∗
-           term_session_frag tB (Session Resp kA kB (Some tA))
+           session_auth nsl_name tA (SessionData Init kA kB (Some tB)) ∗
+           session_frag nsl_name tB (SessionData Resp kA kB (Some tA))
          )
        else True) -∗
       Ψ (repr onB)) -∗
@@ -506,7 +205,7 @@ iIntros (?) "#Hctx #HtA unreg #HkA #HkB_lo #HkB_hi Hpost".
 wp_list (_ :: _ :: []).
 wp_term_of_list.
 wp_tenc => /=.
-iMod (nsl_sess_alloc_init lvl kA kB
+iMod (session_alloc_init nsl_name lvl kA kB
         with "Hctx HkA unreg HkB_lo HkB_hi HtA") as "[auth #fragA]"=> //.
 wp_pures; wp_bind (send _); iApply wp_send.
   by iModIntro; iApply termT_msg1.
@@ -525,24 +224,24 @@ rewrite termT_of_list.
 iPoseProof (big_sepL_lookup with "Hm2") as "m2_tA"; first exact: enA'.
 iPoseProof (big_sepL_lookup with "Hm2") as "m2_nB"; first exact: enB.
 iPoseProof (big_sepL_lookup with "Hm2") as "m2_kB"; first exact: epkB'.
-set  sA := Session Init kA kB _.
-pose sB := Session Resp kA kB (Some tA).
-pose sA' := Session Init kA kB (Some nB).
-iAssert (guarded lm2 (term_session_frag nB sB)) as "{fragB} #fragB".
+set  sA := SessionData Init kA kB _.
+pose sB := SessionData Resp kA kB (Some tA).
+pose sA' := SessionData Init kA kB (Some nB).
+iAssert (guarded lm2 (session_frag nsl_name nB sB)) as "{fragB} #fragB".
   case: lm2 => //=.
   iDestruct "fragB" as (nA' nB' kB') "/= (%em2 & fragB)".
   move/Spec.of_list_inj in em2; subst m2.
   by case: enA' epkB' enB => [] -> [] -> [] -> {nA' nB' kB'}.
 iClear (enA' enB epkB') "Hm2".
 iPoseProof (stermTP with "HtA m2_tA") as "{m2_tA} %Hlm2".
-iMod (term_session_session_inv1 with "Hctx fragB") as "#sessB" => //.
+iMod (session_frag_session_inv1 with "Hctx fragB") as "#sessB" => //.
 iAssert (▷ ⌜lm2 = lvl⌝)%I as "e".
   iModIntro.
   case: lvl lm2 Hlm2 => [] // [] //= _.
   iDestruct "sessB" as "(_&_&_&_&HtA')".
   by iApply (stermT_agree with "HtA' HtA").
 wp_pures; iDestruct "e" as "->".
-iMod (nsl_sess_update with "Hctx auth fragB") as "{fragA} [auth #fragA]" => //.
+iMod (session_update with "Hctx auth fragB") as "{fragA} [auth #fragA]" => //.
 set m3 := TEnc _ _.
 wp_bind (send _); iApply wp_send.
   iModIntro.
@@ -558,7 +257,7 @@ Qed.
 Lemma wp_responder kB E Ψ :
   ↑cryptoN.@"nsl" ⊆ E →
   nsl_ctx -∗
-  nsl_key Resp kB -∗
+  nsl_key_inv Resp kB -∗
   (∀ ot : option (term * term * term),
       (if ot is Some (pkA, nA, nB) then
          ∃ lvl kA,
@@ -567,8 +266,8 @@ Lemma wp_responder kB E Ψ :
            stermT lvl nA ∗
            stermT lvl nB ∗
            guarded lvl (
-            term_session_frag nA (Session Init kA kB (Some nB)) ∗
-            term_session_auth nB (Session Resp kA kB (Some nA)))
+            session_frag nsl_name nA (SessionData Init kA kB (Some nB)) ∗
+            session_auth nsl_name nB (SessionData Resp kA kB (Some nA)))
        else True) -∗
        Ψ (repr ot)) -∗
   WP responder (TKey Dec kB) (TKey Enc kB) #() @ E {{ Ψ }}.
@@ -589,23 +288,25 @@ iDestruct (termT_tag_adec_pub_sec with "Hm1 []") as (lm1) "{Hm1} [Hm1 fragA]"; e
 rewrite termT_of_list.
 iPoseProof (big_sepL_lookup with "Hm1") as "HnA"; first exact: enA.
 iPoseProof (big_sepL_lookup with "Hm1") as "HpkA"; first exact: epkA.
-pose Pm1 := term_session_frag nA (Session Init kA kB None).
+pose (Pm1 := session_frag nsl_name nA (SessionData Init kA kB None)).
 iAssert (guarded lm1 Pm1) as "{fragA} fragA".
   iApply (guarded_mono with "fragA").
   iIntros "!> {fragA} #fragA".
   iDestruct "fragA" as (nA' kA') "/= [%em1 #fragA]".
   move/Spec.of_list_inj in em1; subst m1.
   by case: enA epkA => [] -> [] -> {nA' kA'}.
-iMod (term_session_session_inv2 with "Hctx HnA fragA") as "{HnA} #HnA" => //.
-iMod (@term_session_session_inv3 _ _ _ (Session Init kA _ _) with "Hctx HpkA fragA") as "#HkA_lo" => //=.
-iMod (term_session_session_inv4 with "Hctx fragA") as "#HkA_hi" => //.
+iMod (session_frag_session_inv2 with "Hctx HnA fragA") as "{HnA} #HnA" => //.
+iMod (session_frag_key_inv with "Hctx fragA") as "#HkA_hi" => //.
+iAssert (▷ termT Pub (TKey Enc kA))%I as "#HkA_lo".
+  case: lm1=> //=; iModIntro.
+  by iDestruct "HkA_hi" as "(?&?)".
 wp_pures; wp_bind (gen _); iApply (wp_gen _ lm1); iIntros (nB) "unreg #HnB".
 wp_pures.
 wp_list (_ :: _ :: _ :: []); wp_term_of_list. 
 wp_tenc; wp_pures.
 set m2 := Spec.of_list [nA; nB; TKey Enc kB].
-set sB := Session Resp kA kB (Some nA).
-iMod (nsl_sess_alloc_resp _ kA kB nA with "Hctx HkB unreg HkA_lo HkA_hi HnB HnA")
+set sB := SessionData Resp kA kB (Some nA).
+iMod (session_alloc_resp _ _ kA kB nA with "Hctx HkB unreg HkA_lo HkA_hi HnB HnA")
     as "[auth #fragB]"=> //=.
 wp_bind (send _); iApply wp_send.
   iModIntro.
@@ -629,9 +330,9 @@ iApply ("Hpost" $! (Some (_, _, _))).
 iExists _, _; do 4![iSplit => //].
 case: lm1 => //=.
 iDestruct "Hprot3" as (nA' kA') "[#frag1 #frag2]".
-set sB' := (Session Resp kA' _ _).
-iPoseProof (term_session_agree with "auth frag2") as "%sess".
-have [-> ->] : sB' = sB by apply: to_session_included_eq => //=; eauto.
+set sB' := (SessionData Resp kA' _ _).
+iPoseProof (session_agree with "auth frag2") as "%sess".
+have [-> ->] : sB' = sB by apply: to_session_data'_included_eq => //=; eauto.
 by iSplit=> //.
 Qed.
 
